Phi_System/Phi_BI.thy
@@ -3383,7 +3383,8 @@ ML \<open>
 (* (\<And>x. X x \<t>\<r>\<a>\<n>\<s>\<f>\<o>\<r>\<m>\<s> ?Y \<w>\<i>\<t>\<h> P) where ?Y is a variable.
    When X contains some quantified variables \<open>x\<close> that do not parameterize ?Y, the procedure
    existentially quantifies X, and assign \<open>\<exists>x. X x\<close> to ?Y.
-   cannot work on \<open>_ \<^emph>[_] _\<close> (*TODO*)
+   cannot work on \<open>_ \<^emph>[_] _\<close> (*TODO, but the thing is there is no type embedding of existence,
+                                     unless we use \<Sigma> and \<S>, but... mmmmm.... well, a lot of work.*)
  *)
 fun apply_refl_by_unifying (refl, exintro', Gx, Gy) ctxt thm =
   let val (vs, _, goal) = Phi_Help.leading_antecedent (Thm.prop_of thm)
@@ -3449,10 +3450,10 @@ fun apply_refl_by_unifying (refl, exintro', Gx, Gy) ctxt thm =
 text \<open>Here, we assign the semantics of schematic variables occurring in targets and sources to be,
   a wild-card for any single separation item.\<close>
 
-declare transformation_refl_assigning_W [\<phi>reason %ToA_assigning_var for \<open>_ \<Ztypecolon> ?var \<^emph>[_] _ \<t>\<r>\<a>\<n>\<s>\<f>\<o>\<r>\<m>\<s> _ \<Ztypecolon> (_ \<^emph> _) \<^emph>[_] _ \<w>\<i>\<t>\<h> _\<close>]
-        transformation_refl_assigning_R [\<phi>reason %ToA_assigning_var for \<open>_ \<Ztypecolon> (_ \<^emph> _) \<^emph>[_] _ \<t>\<r>\<a>\<n>\<s>\<f>\<o>\<r>\<m>\<s> _ \<Ztypecolon> ?var \<^emph>[_] _ \<w>\<i>\<t>\<h> _\<close>]
-        transformation_refl_with_WR [\<phi>reason %ToA_assigning_var+1 for \<open>_ \<Ztypecolon> ?var \<^emph>[False] _ \<t>\<r>\<a>\<n>\<s>\<f>\<o>\<r>\<m>\<s> _ \<Ztypecolon> _ \<^emph>[_] _ \<w>\<i>\<t>\<h> _\<close>
-                                                                 \<open>_ \<Ztypecolon> _ \<^emph>[_] _ \<t>\<r>\<a>\<n>\<s>\<f>\<o>\<r>\<m>\<s> _ \<Ztypecolon> ?var \<^emph>[False] _ \<w>\<i>\<t>\<h> _\<close>]
+declare transformation_refl_assigning_W [\<phi>reason %ToA_assigning_var for \<open>_ \<Ztypecolon> ?var \<^emph>[True] _ \<t>\<r>\<a>\<n>\<s>\<f>\<o>\<r>\<m>\<s> _ \<Ztypecolon> (_ \<^emph> _) \<^emph>[_] _ \<w>\<i>\<t>\<h> _\<close>]
+        transformation_refl_assigning_R [\<phi>reason %ToA_assigning_var for \<open>_ \<Ztypecolon> (_ \<^emph> _) \<^emph>[_] _ \<t>\<r>\<a>\<n>\<s>\<f>\<o>\<r>\<m>\<s> _ \<Ztypecolon> ?var \<^emph>[True] _ \<w>\<i>\<t>\<h> _\<close>]
+        transformation_refl_with_WR [\<phi>reason %ToA_assigning_var+1 for \<open>_ \<Ztypecolon> ?var \<^emph>[_] _ \<t>\<r>\<a>\<n>\<s>\<f>\<o>\<r>\<m>\<s> _ \<Ztypecolon> _ \<^emph>[_] _ \<w>\<i>\<t>\<h> _\<close>
+                                                                      \<open>_ \<Ztypecolon> _ \<^emph>[_] _ \<t>\<r>\<a>\<n>\<s>\<f>\<o>\<r>\<m>\<s> _ \<Ztypecolon> ?var \<^emph>[_] _ \<w>\<i>\<t>\<h> _\<close>]
 (*
 lemma [\<phi>reason 4100 for \<open>_ \<t>\<r>\<a>\<n>\<s>\<f>\<o>\<r>\<m>\<s> _ \<Ztypecolon> ?var_U \<^emph>[_] _ \<w>\<i>\<t>\<h> _\<close>
                         \<open>_ \<Ztypecolon> ?var_T \<^emph>[_] _ \<t>\<r>\<a>\<n>\<s>\<f>\<o>\<r>\<m>\<s> _ \<Ztypecolon> _ \<^emph>[_] _ \<w>\<i>\<t>\<h> _\<close>
